generational/spec/GC.Gen.ChunkedCheney.fst
@@ -1,0 +1,319 @@
+/// ---------------------------------------------------------------------------
+/// GC.Gen.ChunkedCheney -- Chunked-major Cheney forwarding core
+/// ---------------------------------------------------------------------------
+
+module GC.Gen.ChunkedCheney
+
+open FStar.Seq
+module U64 = FStar.UInt64
+
+open GC.Spec.Base
+open GC.Gen.MinorHeap
+open GC.Gen.Promote
+
+module MH = GC.Spec.MajorHeap
+module SpecAlloc = GC.Spec.Allocator
+module ChunkedPromote = GC.Gen.ChunkedPromote
+module Dense = GC.Gen.Cheney
+module AllocProps = GC.Gen.AllocProps
+
+let single_chunk_cheney_state (cs: Dense.cheney_state)
+  : GTot chunked_cheney_state =
+  { ccs_major = MH.single_chunk_major_heap cs.cs_major;
+    ccs_fp    = cs.cs_fp;
+    ccs_fwd   = cs.cs_fwd;
+    ccs_queue = cs.cs_queue }
+
+let chunked_cheney_forward_normal
+  (minor: minor_state) (cs: chunked_cheney_state) (addr: U64.t)
+  (fuel: nat)
+  : GTot chunked_cheney_state =
+  if not (Seq.mem addr (minor_objects minor)) || cs.ccs_fwd addr <> 0UL
+  then cs
+  else
+    let wz = minor_wosize minor addr in
+    if wz = 0 then cs
+    else
+      let res =
+        ChunkedPromote.chunked_promote_object_with_fuel
+          minor cs.ccs_major addr cs.ccs_fp wz fuel in
+      if res.new_addr = 0UL then cs
+      else
+        { ccs_major = res.major_out;
+          ccs_fp    = res.fp_out;
+          ccs_fwd   = extend_forwarding cs.ccs_fwd addr res.new_addr;
+          ccs_queue = Seq.append cs.ccs_queue (Seq.create 1 addr) }
+
+let chunked_cheney_forward_one
+  (minor: minor_state) (cs: chunked_cheney_state) (addr: U64.t)
+  (fuel: nat)
+  : GTot chunked_cheney_state =
+  if cs.ccs_fwd addr <> 0UL then cs
+  else if is_infix_in_minor minor addr then
+    let parent = infix_parent minor addr in
+    let cs' = chunked_cheney_forward_normal minor cs parent fuel in
+    if cs'.ccs_fwd parent <> 0UL &&
+       U64.v addr >= U64.v parent &&
+       U64.v (cs'.ccs_fwd parent) + (U64.v addr - U64.v parent) < heap_size
+    then
+      let delta = U64.v addr - U64.v parent in
+      { cs' with ccs_fwd = extend_forwarding cs'.ccs_fwd addr
+                              (U64.uint_to_t
+                                (U64.v (cs'.ccs_fwd parent) + delta)) }
+    else cs'
+  else
+    chunked_cheney_forward_normal minor cs addr fuel
+
+let chunked_cheney_forward_normal_noop
+  (minor: minor_state) (cs: chunked_cheney_state) (addr: U64.t)
+  (fuel: nat)
+  : Lemma (requires ~(Seq.mem addr (minor_objects minor)) \/
+                    cs.ccs_fwd addr <> 0UL)
+          (ensures chunked_cheney_forward_normal minor cs addr fuel == cs)
+  = ()
+
+let chunked_cheney_forward_normal_noop_wz0
+  (minor: minor_state) (cs: chunked_cheney_state) (addr: U64.t)
+  (fuel: nat)
+  : Lemma (requires Seq.mem addr (minor_objects minor) /\
+                    cs.ccs_fwd addr = 0UL /\
+                    minor_wosize minor addr = 0)
+          (ensures chunked_cheney_forward_normal minor cs addr fuel == cs)
+  = ()
+
+let chunked_cheney_forward_normal_noop_oom
+  (minor: minor_state) (cs: chunked_cheney_state) (addr: U64.t)
+  (fuel: nat)
+  : Lemma
+      (requires Seq.mem addr (minor_objects minor) /\
+                cs.ccs_fwd addr = 0UL /\
+                minor_wosize minor addr > 0 /\
+                (ChunkedPromote.chunked_promote_object_with_fuel
+                  minor cs.ccs_major addr cs.ccs_fp
+                  (minor_wosize minor addr) fuel).new_addr = 0UL)
+      (ensures chunked_cheney_forward_normal minor cs addr fuel == cs)
+  = ()
+
+let chunked_cheney_forward_normal_success
+  (minor: minor_state) (cs: chunked_cheney_state) (addr: U64.t)
+  (fuel: nat)
+  : Lemma
+      (requires Seq.mem addr (minor_objects minor) /\
+                cs.ccs_fwd addr = 0UL /\
+                minor_wosize minor addr > 0 /\
+                (ChunkedPromote.chunked_promote_object_with_fuel
+                  minor cs.ccs_major addr cs.ccs_fp
+                  (minor_wosize minor addr) fuel).new_addr <> 0UL)
+      (ensures
+        (let wz = minor_wosize minor addr in
+         let res =
+           ChunkedPromote.chunked_promote_object_with_fuel
+             minor cs.ccs_major addr cs.ccs_fp wz fuel in
+         chunked_cheney_forward_normal minor cs addr fuel ==
+         { ccs_major = res.major_out;
+           ccs_fp    = res.fp_out;
+           ccs_fwd   = extend_forwarding cs.ccs_fwd addr res.new_addr;
+           ccs_queue = Seq.append cs.ccs_queue (Seq.create 1 addr) }))
+  = ()
+
+let chunked_cheney_forward_normal_other_fwd
+  (minor: minor_state) (cs: chunked_cheney_state) (addr: U64.t)
+  (y: U64.t) (fuel: nat)
+  : Lemma (requires y <> addr)
+          (ensures
+            (chunked_cheney_forward_normal minor cs addr fuel).ccs_fwd y ==
+            cs.ccs_fwd y)
+  = ()
+
+let chunked_cheney_forward_one_noop
+  (minor: minor_state) (cs: chunked_cheney_state) (addr: U64.t)
+  (fuel: nat)
+  : Lemma (requires cs.ccs_fwd addr <> 0UL \/
+                    (~(Seq.mem addr (minor_objects minor)) /\
+                     ~(is_infix_in_minor minor addr)))
+          (ensures chunked_cheney_forward_one minor cs addr fuel == cs)
+  = ()
+
+let chunked_cheney_forward_one_normal
+  (minor: minor_state) (cs: chunked_cheney_state) (addr: U64.t)
+  (fuel: nat)
+  : Lemma (requires cs.ccs_fwd addr = 0UL /\
+                    ~(is_infix_in_minor minor addr))
+          (ensures
+            chunked_cheney_forward_one minor cs addr fuel ==
+            chunked_cheney_forward_normal minor cs addr fuel)
+  = ()
+
+let chunked_cheney_forward_one_infix
+  (minor: minor_state) (cs: chunked_cheney_state) (addr: U64.t)
+  (fuel: nat)
+  : Lemma (requires cs.ccs_fwd addr = 0UL /\
+                    is_infix_in_minor minor addr /\
+                    U64.v addr >= U64.v (infix_parent minor addr))
+          (ensures
+            (let parent = infix_parent minor addr in
+             let cs' = chunked_cheney_forward_normal minor cs parent fuel in
+             let r = chunked_cheney_forward_one minor cs addr fuel in
+             r.ccs_major == cs'.ccs_major /\
+             r.ccs_fp == cs'.ccs_fp /\
+             r.ccs_queue == cs'.ccs_queue))
+  = ()
+
+let chunked_cheney_forward_one_infix_guard_pass
+  (minor: minor_state) (cs: chunked_cheney_state) (addr: U64.t)
+  (fuel: nat)
+  : Lemma (requires cs.ccs_fwd addr = 0UL /\
+                    is_infix_in_minor minor addr /\
+                    (let parent = infix_parent minor addr in
+                     let cs' =
+                       chunked_cheney_forward_normal minor cs parent fuel in
+                     cs'.ccs_fwd parent <> 0UL /\
+                     U64.v addr >= U64.v parent /\
+                     U64.v (cs'.ccs_fwd parent) +
+                       (U64.v addr - U64.v parent) < heap_size))
+          (ensures
+            (let parent = infix_parent minor addr in
+             let cs' = chunked_cheney_forward_normal minor cs parent fuel in
+             let delta = U64.v addr - U64.v parent in
+             let sum = U64.uint_to_t (U64.v (cs'.ccs_fwd parent) + delta) in
+             let r = chunked_cheney_forward_one minor cs addr fuel in
+             r.ccs_fwd == extend_forwarding cs'.ccs_fwd addr sum /\
+             r.ccs_major == cs'.ccs_major /\
+             r.ccs_fp == cs'.ccs_fp /\
+             r.ccs_queue == cs'.ccs_queue))
+  = ()
+
+let chunked_cheney_forward_one_infix_guard_fail
+  (minor: minor_state) (cs: chunked_cheney_state) (addr: U64.t)
+  (fuel: nat)
+  : Lemma (requires cs.ccs_fwd addr = 0UL /\
+                    is_infix_in_minor minor addr /\
+                    (let parent = infix_parent minor addr in
+                     let cs' =
+                       chunked_cheney_forward_normal minor cs parent fuel in
+                     ~(cs'.ccs_fwd parent <> 0UL &&
+                       U64.v addr >= U64.v parent &&
+                       U64.v (cs'.ccs_fwd parent) +
+                         (U64.v addr - U64.v parent) < heap_size)))
+          (ensures
+            chunked_cheney_forward_one minor cs addr fuel ==
+            chunked_cheney_forward_normal minor cs
+              (infix_parent minor addr) fuel)
+  = ()
+
+#push-options "--z3rlimit 5 --fuel 0 --ifuel 0 --split_queries always"
+let chunked_cheney_forward_normal_default_single_chunk_compat
+  (minor: minor_state) (cs: Dense.cheney_state) (addr: U64.t)
+  : Lemma
+      (ensures
+        chunked_cheney_forward_normal
+          minor (single_chunk_cheney_state cs) addr
+          SpecAlloc.alloc_search_fuel ==
+        single_chunk_cheney_state
+          (Dense.cheney_forward_normal minor cs addr))
+  =
+  if not (Seq.mem addr (minor_objects minor)) || cs.cs_fwd addr <> 0UL
+  then begin
+    Dense.cheney_forward_normal_noop minor cs addr;
+    chunked_cheney_forward_normal_noop
+      minor (single_chunk_cheney_state cs) addr
+      SpecAlloc.alloc_search_fuel
+  end
+  else
+    let wz = minor_wosize minor addr in
+    if wz = 0 then begin
+      Dense.cheney_forward_normal_noop_wz0 minor cs addr;
+      chunked_cheney_forward_normal_noop_wz0
+        minor (single_chunk_cheney_state cs) addr
+        SpecAlloc.alloc_search_fuel
+    end
+    else begin
+      AllocProps.alloc_spec_obj_valid cs.cs_major cs.cs_fp wz;
+      ChunkedPromote.chunked_promote_object_with_fuel_single_chunk_compat
+        minor cs.cs_major addr cs.cs_fp wz SpecAlloc.alloc_search_fuel;
+      let dense_res = promote_object minor cs.cs_major addr cs.cs_fp wz in
+      let chunked_res =
+        ChunkedPromote.chunked_promote_object_with_fuel
+          minor (MH.single_chunk_major_heap cs.cs_major) addr cs.cs_fp wz
+          SpecAlloc.alloc_search_fuel in
+      assert (chunked_res.major_out ==
+              MH.single_chunk_major_heap dense_res.major_out);
+      assert (chunked_res.fp_out == dense_res.fp_out);
+      assert (chunked_res.new_addr == dense_res.new_addr);
+      if dense_res.new_addr = 0UL then begin
+        Dense.cheney_forward_normal_noop_oom minor cs addr;
+        chunked_cheney_forward_normal_noop_oom
+          minor (single_chunk_cheney_state cs) addr
+          SpecAlloc.alloc_search_fuel
+      end
+      else begin
+        Dense.cheney_forward_normal_success minor cs addr;
+        chunked_cheney_forward_normal_success
+          minor (single_chunk_cheney_state cs) addr
+          SpecAlloc.alloc_search_fuel
+      end
+    end
+#pop-options
+
+#push-options "--z3rlimit 5 --fuel 0 --ifuel 0 --split_queries always"
+let chunked_cheney_forward_one_default_single_chunk_compat
+  (minor: minor_state) (cs: Dense.cheney_state) (addr: U64.t)
+  : Lemma
+      (ensures
+        chunked_cheney_forward_one
+          minor (single_chunk_cheney_state cs) addr
+          SpecAlloc.alloc_search_fuel ==
+        single_chunk_cheney_state
+          (Dense.cheney_forward_one minor cs addr))
+  =
+  if cs.cs_fwd addr <> 0UL then begin
+    Dense.cheney_forward_one_noop minor cs addr;
+    chunked_cheney_forward_one_noop
+      minor (single_chunk_cheney_state cs) addr
+      SpecAlloc.alloc_search_fuel
+  end
+  else if is_infix_in_minor minor addr then begin
+    let parent = infix_parent minor addr in
+    chunked_cheney_forward_normal_default_single_chunk_compat minor cs parent;
+    let dense_parent = Dense.cheney_forward_normal minor cs parent in
+    let chunked_parent =
+      chunked_cheney_forward_normal
+        minor (single_chunk_cheney_state cs) parent
+        SpecAlloc.alloc_search_fuel in
+    assert (chunked_parent == single_chunk_cheney_state dense_parent);
+    assert (chunked_parent.ccs_fwd == dense_parent.cs_fwd);
+    assert (chunked_parent.ccs_major ==
+            MH.single_chunk_major_heap dense_parent.cs_major);
+    assert (chunked_parent.ccs_fp == dense_parent.cs_fp);
+    assert (chunked_parent.ccs_queue == dense_parent.cs_queue);
+    if dense_parent.cs_fwd parent <> 0UL &&
+       U64.v addr >= U64.v parent &&
+       U64.v (dense_parent.cs_fwd parent) + (U64.v addr - U64.v parent) < heap_size
+    then begin
+      assert (chunked_parent.ccs_fwd parent <> 0UL);
+      assert (U64.v (chunked_parent.ccs_fwd parent) ==
+              U64.v (dense_parent.cs_fwd parent));
+      Dense.cheney_forward_one_infix_guard_pass minor cs addr;
+      chunked_cheney_forward_one_infix_guard_pass
+        minor (single_chunk_cheney_state cs) addr
+        SpecAlloc.alloc_search_fuel
+    end
+    else begin
+      assert (~(chunked_parent.ccs_fwd parent <> 0UL &&
+                U64.v addr >= U64.v parent &&
+                U64.v (chunked_parent.ccs_fwd parent) +
+                  (U64.v addr - U64.v parent) < heap_size));
+      Dense.cheney_forward_one_infix_guard_fail minor cs addr;
+      chunked_cheney_forward_one_infix_guard_fail
+        minor (single_chunk_cheney_state cs) addr
+        SpecAlloc.alloc_search_fuel
+    end
+  end
+  else begin
+    Dense.cheney_forward_one_normal minor cs addr;
+    chunked_cheney_forward_one_normal
+      minor (single_chunk_cheney_state cs) addr
+      SpecAlloc.alloc_search_fuel;
+    chunked_cheney_forward_normal_default_single_chunk_compat minor cs addr
+  end
+#pop-options
